%
% Copyright Â© 2016 Peeter Joot.  All Rights Reserved.
% Licenced as described in the file LICENSE under the root directory of this GIT repository.
%
\makeproblem{Dot product expansion of two bivectors.}{problem:multiplication:bivectorDot}{
Show that

\boxedEquation{eqn:bivectorDot:20}{
(\Ba \wedge \Bb) \cdot (\Bc \wedge \Bd)
=
\lr{ (\Ba \wedge \Bb) \cdot \Bc} \cdot \Bd,
}

and hence
\boxedEquation{eqn:bivectorDot:40}{
(\Ba \wedge \Bb) \cdot (\Bc \wedge \Bd)
=
(\Bb \cdot \Bc) (\Ba \cdot \Bd)
-(\Ba \cdot \Bc)( \Bb \cdot \Bd).
}
} % problem

\makeanswer{problem:multiplication:bivectorDot}{
FIXME: this proof relies on triple wedge products, which haven't been introduced yet.  Can rephrase using grade-3 selection.
Also rework as non-problem.
\begin{dmath}\label{eqn:bivectorDot:60}
(\Ba \wedge \Bb) \cdot (\Bc \wedge \Bd)
=
\gpgradezero{
(\Ba \wedge \Bb) (\Bc \wedge \Bd)
}
=
\gpgradezero{
(\Ba \wedge \Bb) (\Bc \Bd - \cancel{\Bc \cdot \Bd})
}
=
\gpgradezero{
\lr{
(\Ba \wedge \Bb) \cdot \Bc
+ \cancel{(\Ba \wedge \Bb) \wedge \Bc }
}
\Bd
}
=
\gpgradezero{
((\Ba \wedge \Bb) \cdot \Bc ) \cdot \Bd
+
\cancel{((\Ba \wedge \Bb) \cdot \Bc ) \wedge \Bd}
}
=
((\Ba \wedge \Bb) \cdot \Bc ) \cdot \Bd.
\end{dmath}

Above, any product that could not possibly contribute a scalar grade has been cancelled.  The remains are now straightforward to expand

\begin{dmath}\label{eqn:bivectorDot:80}
((\Ba \wedge \Bb) \cdot \Bc ) \cdot \Bd
=
(
\Ba (\Bb \cdot \Bc)
-
\Bb (\Ba \cdot \Bc)
)
\cdot \Bd
=
(\Ba \cdot \Bd) (\Bb \cdot \Bc)
-
(\Bb \cdot \Bd) (\Ba \cdot \Bc).
\end{dmath}

} % answer
